src/high/protocols.v
@@ -1,0 +1,16 @@
+
+From iris.proofmode Require Import reduction monpred tactics.
+
+From self.high Require Import dprop dprop_liftings resources modalities post_crash_modality.
+From self.lang Require Import lang.
+From self.high Require Import abstract_state_instances protocol.
+
+Section constant_prot.
+  Context `{nvmG Σ}.
+
+  Program Definition constant_prot (v1 : val) : LocationProtocol unit :=
+    {| pred := λ _ v2, ⌜ v1 = v2 ⌝%I;
+       bumper := id |}.
+  Next Obligation. iIntros. by iApply post_crash_flush_pure. Qed.
+
+End constant_prot.
